Some theorems modified

src/site/discrete/coq-competitions/ee_piirk_2020_11_3.v
@@ -21,14 +21,14 @@ Require Import Arith Psatz.
 Require Import ZArith.
 Require Import Znumtheory.
 Require Import BinInt.
-
-
 Require Import BinIntDef.
 Require Export BinNums.
 Require Import BinPos BinNat.
 
-
 Require Import Datatypes.
+Require Import Decimal DecimalFacts.
+Require Import DecimalNat.
+
 
 Add LoadPath "/home/kalvis/workspace-osx/coq/theory/Init".
 
@@ -36,4 +36,119 @@ Add LoadPath "/home/kalvis/workspace-osx/coq/theory/Init".
 https://blog.zhen-zhang.com/2016/09/19/coq-dev.html
 Require Import Decimal.
 *)
+
+Definition a:nat := 3%nat.
+
+Definition b:uint := (D8 Nil).
+
+Open Scope nat_scope.
+
+Definition hd d :=
+ match d with
+ | Nil => 0
+ | D0 _ => 0
+ | D1 _ => 1
+ | D2 _ => 2
+ | D3 _ => 3
+ | D4 _ => 4
+ | D5 _ => 5
+ | D6 _ => 6
+ | D7 _ => 7
+ | D8 _ => 8
+ | D9 _ => 9
+end.
+
+Definition tl d :=
+ match d with
+ | Nil => d
+ | D0 d | D1 d | D2 d | D3 d | D4 d | D5 d | D6 d | D7 d | D8 d | D9 d => d
+end.
+
+(** Number of digits *)
+Fixpoint usize (d:uint) : nat :=
+  match d with
+  | Nil => 0
+  | D0 d => S (usize d)
+  | D1 d => S (usize d)
+  | D2 d => S (usize d)
+  | D3 d => S (usize d)
+  | D4 d => S (usize d)
+  | D5 d => S (usize d)
+  | D6 d => S (usize d)
+  | D7 d => S (usize d)
+  | D8 d => S (usize d)
+  | D9 d => S (usize d)
+  end.
+
+(*
+Fixpoint to_lu n :=
+ match n with
+ | 0 => Decimal.zero
+ | S n => Little.succ (to_lu n)
+ end.
+*)
+
+Fixpoint append (L1 L2 : uint) : uint :=
+  match L1 with
+  | Nil => L2
+  | D0 d => D0 (append d L2)
+  | D1 d => D1 (append d L2)
+  | D2 d => D2 (append d L2)
+  | D3 d => D3 (append d L2)
+  | D4 d => D4 (append d L2)
+  | D5 d => D5 (append d L2)
+  | D6 d => D6 (append d L2)
+  | D7 d => D7 (append d L2)
+  | D8 d => D8 (append d L2)
+  | D9 d => D9 (append d L2)
+  end.
+
+Compute (append 200%uint 2002%uint).
+
+
+
+Notation "x ++ y" := (append x y)
+                     (right associativity, at level 60).
+
+
+Fixpoint rev (d:uint) : uint :=
+  match d with
+  | Nil => Nil
+  | D0 d => append (rev d) (D0 Nil)
+  | D1 d => append (rev d) (D1 Nil)
+  | D2 d => append (rev d) (D2 Nil)
+  | D3 d => append (rev d) (D3 Nil)
+  | D4 d => append (rev d) (D4 Nil)
+  | D5 d => append (rev d) (D5 Nil)
+  | D6 d => append (rev d) (D6 Nil)
+  | D7 d => append (rev d) (D7 Nil)
+  | D8 d => append (rev d) (D8 Nil)
+  | D9 d => append (rev d) (D9 Nil)
+  end.
+
+
+Compute (rev 1234%uint).
+
+Compute (usize (to_uint 2002)).
+Compute (of_uint (D8 (D9 Nil))).
+Compute (of_uint (Nil)).
+
+Compute (to_uint 2020%nat).
+
+
+Lemma sample2: exists a:uint, usize a = 2 /\ rev a = a.
+Proof. 
+  exists 22%uint.
+  split. 
+  simpl. reflexivity.
+  simpl. reflexivity.
+Qed.
+
+Theorem ee_piirk_2020_11_3: forall a b:nat, 
+  usize (to_uint a) = 2 -> 
+    usize (to_uint b) = 2 -> 
+      of_uint (rev (to_uint (a + b))) <> a*b.
+Proof. 
+  Admitted.
+
 
