src/site/discrete/coq-competitions/r-scripts/ee-piirk-2020-11-3.R
@@ -1,0 +1,26 @@
+#xx <- rep(365,times=50)
+#yy <- 365:(365-50+1)
+#zz <- yy/xx
+#tt <- cumprod(zz)
+#plot(tt)
+#grid()
+
+
+
+for (a in 10:99) {
+  for (b in 10:99) {
+    if (a*b < 1000) {
+      s <- a+b
+      p <- sprintf("%d",a*b)
+      pinv <- sprintf("%s%s%s",
+                      substring(p,1,1),
+                      substring(p,2,2),
+                      substring(p,3,3))
+      pinv2 <- as.numeric(pinv)
+      if (abs(s - pinv2) ==119) {
+        print(sprintf("(a,b)=(%d,%d)",a,b))
+      }
+    }
+  }
+}
+
